src/common/ASTExtra.v
@@ -1,0 +1,7 @@
+From compcert Require Import AST.
+
+Definition find_named_func {F V} (ge : Genv.t F V) name :=
+  match Genv.find_symbol ge name with
+  | Some blk => Genv.find_funct_ptr ge blk
+  | None => None
+  end.
